Add PLF dependency

midterm-practice/Sample_Midterm_Solutions1.v
@@ -1,10 +1,10 @@
 (* Sample Midterm for CS 565 Do not redistribute!
 
 As a refresher, here is a summary of the learning outcomes from the
-first seven weeks of the course: The midterm will cover the first seven
+first seven weeks of the course: The midterm will cover the first six
 weeks-- the midterm will not cover denotational semantics. *)
 
-(* W1:
+(*  W1:
 Write simple functional programs.
 Represent the syntax of program as an inductive datatype.
 Implement interpreters for a simple language as a recursive function.
@@ -51,43 +51,35 @@ Identify sufficient conditions for the existence of the fixpoint of a function, 
   Part 1: Basic Functional Programming
  *********************************************************)
 
+From LF Require Export Poly.
 From LF Require Export Imp.
 From Coq Require Import Lists.List.
 From Coq Require Import Strings.String.
 From Coq Require Import Lia.
 Import ListNotations.
 
-(** Exercise:  *)
 (* Define a polymorphic [remove] function that removes the nth element
    from a list. if the index is beyond the end of the list, the original
    list is returned. *)
-Fixpoint remove {A : Type} (l : list A) (n : nat) : list A := l.
 
-(** Exercise:  *)
-Example remove_ex1 : remove [1; 3; 5; 7] 2 = [1; 3; 7].
-  (* FILL IN HERE *)
-Admitted.
+Fixpoint remove {A : Type} (l : list A) (n : nat) : list A :=
+  match n, l with
+    0, a :: l' => l'
+  | S n', a :: l' => a :: (remove l' n')
+  | _, _ => nil
+  end.
 
-(** Exercise:  *)
-Example remove_ex2 : remove [1; 3; 5; 7] 5 = [1; 3; 5; 7].
-  (* FILL IN HERE *)
-Admitted.
+Example remove_ex1 : remove [1; 3; 5; 7] 2 = [1; 3; 7]. reflexivity. Qed.
+Example remove_ex2 : remove [1; 3; 5; 7] 5 = [1; 3; 5; 7]. reflexivity. Qed.
+Example remove_ex3 : remove [1; 3; 5; 7] 0 = [3; 5; 7]. reflexivity. Qed.
+Lemma remove_2 {A} : forall (l : list A), remove l 0 = tl l. destruct l; reflexivity. Qed.
 
-(** Exercise:  *)
-Example remove_ex3 : remove [1; 3; 5; 7] 0 = [3; 5; 7].
-  (* FILL IN HERE *)
-Admitted.
-
-(** Exercise:  *)
-Lemma remove_2 {A} : forall (l : list A), remove l 0 = tl l.
-  (* FILL IN HERE *)
-Admitted.
 
 Module BSTs.
   (* Maps with numeric keys can be implemented with binary search trees
    (BSTs). Insert and lookup operations on BSTs take time proportional
    to the height of the tree.  If you don't recall BSTs or haven't
-   seen them in a while, see Wikipedia. *)
+   seen them in a while, see Wikipedia. Define *)
 
   Inductive Tree (V : Type) : Type :=
   | leaf
@@ -113,43 +105,39 @@ Module BSTs.
     are less than [k] and all the values of the right subtree are
     greater than [k]. *)
 
-  (** Exercise: *)
+  Notation "x =? y" := (Nat.eqb x y) : nat_scope.
+  Notation "x <=? y" := (Nat.leb x y) : nat_scope.
+
   (* Define a lookup operation on well-formed BSTs.
    [lookup k t] is the value assocated with k in t, or None if k is not bound in t. *)
   Fixpoint lookup {V : Type} (k : nat) (t : @Tree V) : option V :=
-    (* Replace this line with your definition. *)  None.
+    match t with
+    | leaf => None
+    | node lt k' v rt => if k =? k' then Some v
+                         else if k <=? k' then lookup k lt
+                              else lookup k rt
+    end.
 
-  (** Exercise: *)
   (* Define an insertion operation on well-formed BSTs: insert k v t
    is the BST updates the value associated with k to v in t, adding it
    if the [k] is not present. *)
+
   Fixpoint insert {V : Type} (k : nat) (v : V) (t : Tree V) : Tree V :=
     match t with
     | leaf => node leaf k v leaf
-    | node lt k' v' rt => if k =? k' then node lt k v rt
+    | node lt k' v' rt => if Nat.eqb k k' then node lt k v rt
                           else if k <=? k' then node (insert k v lt) k' v' rt
                                else node lt k' v' (insert k v rt)
     end.
 
   Open Scope string_scope.
-  (** Exercise: *)
   Example bst_ex1 :
     insert 5 "five" (insert 2 "two" (insert 4 "four" empty_tree)) = ex_tree.
-  Proof.
-    (* FILL IN HERE *)
-  Admitted.
-
-  (** Exercise: *)
+  Proof. reflexivity. Qed.
   Example bst_ex2 : lookup 5 ex_tree = Some "five".
-  Proof.
-    (* FILL IN HERE *)
-  Admitted.
-
-  (** Exercise: *)
+  Proof. reflexivity. Qed.
   Example bst_ex3 : lookup 3 ex_tree = None.
-  Proof.
-    (* FILL IN HERE *)
-  Admitted.
+  Proof. reflexivity. Qed.
 
   (*********************************************************
   Part 2: Inductive Propositions
@@ -165,36 +153,21 @@ Module BSTs.
       lookup [2] in that tree, we get the wrong answer, because
       [lookup] assumes [2] is in the left subtree: *)
 
-  (** Exercise: *)
   Example not_bst_lookup_wrong :
     lookup 2 bad_tree = None.
   Proof.
-    (* FILL IN HERE *)
-  Admitted.
+    reflexivity.
+  Qed.
 
   (** So, let's formalize when a tree is well-formed. To do so, we first
     define a helper [ForallT] to express that idea that a predicate
     holds at every node of a tree: *)
 
-  Fixpoint ForallT {V : Type} (P: nat -> V -> Prop) (t : Tree V) : Prop :=
+  Fixpoint ForallT {V : Type} (P: nat -> V -> Prop) (t: Tree V) : Prop :=
     match t with
     | leaf => True
     | node lt k v rt => P k v /\ ForallT P lt /\ ForallT P rt
     end.
-
-  Inductive ForallT' {V : Type} (P: nat -> V -> Prop) : Tree V -> Prop :=
-  | Forall_leaf : ForallT' P leaf
-  | Forall_node : forall lt k v rt,
-      P k v ->
-      ForallT' P lt ->
-      ForallT' P rt ->
-      ForallT' P (node lt k v rt).
-
-  Lemma silly_ex : 3 <= 2 -> 2 + 2 = 5.
-  Proof.
-    intro.
-    lia.
-  Qed.
 
   (** Second, we define well-formedness of BSTs:
 
@@ -204,92 +177,80 @@ Module BSTs.
       key, its right nodes have a greater key, and the left and right
       subtrees are themselves BSTs. *)
 
-  (** Exercise: *)
-    Inductive BST {V : Type} : Tree V -> Prop :=
-    | BST_leaf : BST leaf
-    | BST_node :
-        forall lt k v rt,
-          ForallT (fun y _ => y < k) lt ->
-          ForallT (fun y _ => k < y) rt ->
-          BST lt ->
-          BST rt ->
-          BST (node lt k v rt).
+  Inductive BST {V : Type} : Tree V -> Prop :=
+  | BST_leaf : BST leaf
+  | BST_node : forall l x v r,
+      ForallT (fun y _ => y < x) l ->
+      ForallT (fun y _ => y > x) r ->
+      BST l ->
+      BST r ->
+      BST (node l x v r).
 
   (** Let's check that [BST] correctly classifies a couple of example
     trees: *)
 
-  (** Exercise: *)
   Example is_BST_ex :
     BST ex_tree.
   Proof.
-    (* FILL IN HERE *)
-  Admitted.
+    unfold ex_tree.
+    repeat (constructor).
+  Qed.
 
-  (* 4
-    / \
-   5  2
-   *)
-
-  (** Exercise: *)
   Example not_BST_ex :
     ~ BST bad_tree.
   Proof.
-    unfold not; intro contra.
-    inversion contra; subst.
-    simpl in H3.
-    lia.
+    unfold bad_tree. intros contra.
+    inversion contra; subst. inversion H3; subst. lia.
   Qed.
 
-  (** Exercise: *)
   (** Prove that the empty tree is a BST. *)
+
   Theorem empty_tree_BST : forall (V : Type),
       BST (@empty_tree V).
   Proof.
-    (* FILL IN HERE *)
-  Admitted.
+    repeat constructor.
+  Qed.
 
+  (** Prove that [insert] produces a BST, assuming it is given one.
 
-  (** Prove that [insert] produces a BST, assuming it is given one. *)
-  (* Start by proving this helper lemma, which says that [insert]
-    preserves any node predicate. *)
+    Start by proving this helper lemma, which says that [insert]
+    preserves any node predicate. Proceed by induction on [t]. *)
 
-  (** Exercise: *)
   Lemma ForallT_insert : forall (V : Type) (P : nat -> V -> Prop) (t : Tree V),
       ForallT P t -> forall (k : nat) (v : V),
         P k v -> ForallT P (insert k v t).
   Proof.
-    (* FILL IN HERE *)
-  Admitted.
+    induction t; simpl; intros.
+    - repeat constructor; assumption.
+    - destruct (k =? key)%nat eqn: ?.
+      + destruct H as [? [? ?] ].
+        simpl; repeat split; try assumption.
+      + destruct (k <=? key)%nat eqn: ?; simpl.
+        * destruct H as [? [? ?] ]; repeat split; try assumption.
+          apply IHt1; assumption.
+        * destruct H as [? [? ?] ]; repeat split; try assumption.
+          apply IHt2; assumption.
+  Qed.
 
-  Open Scope nat_scope.
-
-  (** Exercise: *)
   (** Now prove the main theorem. *)
+
   Theorem insert_BST : forall (V : Type) (k : nat) (v : V) (t : Tree V),
       BST t -> BST (insert k v t).
   Proof.
-    intros ? ? ? ? H.
-    induction H.
+    intros ? ? ? ? H; induction H.
     - simpl; repeat constructor.
-    - simpl.
-      destruct (k =? k0) eqn: ?.
-      + Search Nat.eqb.
-        apply Nat.eqb_eq in Heqb.
-        subst.
-        apply BST_node; assumption.
-      + destruct (k <=? k0) eqn: ?; simpl.
-        * apply BST_node; try assumption.
-          apply ForallT_insert.
-          assumption.
-          apply Nat.eqb_neq in Heqb.
-          Search Nat.leb.
-          apply leb_complete in Heqb0.
+    - simpl; destruct (k =? x)%nat eqn: ?.
+      + apply EqNat.beq_nat_true in Heqb. subst.
+        constructor; try assumption.
+      + apply EqNat.beq_nat_false in Heqb. subst.
+        destruct (k <=? x)%nat eqn: ?; simpl.
+        * constructor; try assumption.
+          apply Compare_dec.leb_complete in Heqb0.
+          apply ForallT_insert; try assumption.
           lia.
-        * apply BST_node; try assumption.
-          apply ForallT_insert.
-          assumption.
-          apply Nat.leb_gt.
-          assumption.
+        * constructor; try assumption.
+          apply Compare_dec.leb_complete_conv in Heqb0.
+          apply ForallT_insert; try assumption.
   Qed.
 
 End BSTs.
@@ -300,83 +261,117 @@ End BSTs.
 
 (* Given the following definition of the "less-than-or-equal" relation
   on natural numbers, prove that the relation is reflexive and
-  transitive and is not necessarily symmetric.  *)
+  transitive and is symmetric.  *)
 
 Require Import Coq.Init.Nat.
 
-(** Exercise: *)
+Inductive le : nat -> nat -> Prop :=
+| le_n : forall n, le n n
+| le_S : forall n m, (le n m) -> (le n (S m)).
+
+Notation "m <= n" := (le m n).
+
 (* (a) Reflexivity *)
+
 Lemma le_refl : forall n, n <= n.
 Proof.
-  (* FILL IN HERE *)
-Admitted.
-
-(** Exercise: *)
-(* (cr) lack of symmetry *)
-Lemma le_not_sym : ~ forall m n, m <= n -> n <= m.
-Proof.
-  unfold not; intro contra.
-  assert (2 <= 1).
-  { apply contra.
-    apply le_S.
-    apply le_n. }
-  lia.
+  econstructor.
 Qed.
 
-(** Exercise: *)
+(* (cr) lack of symmetry *)
+
+Lemma le_not_sym : ~ forall m n, m <= n -> n <= m.
+Proof.
+  unfold not.
+  intros.
+  assert (2 <= 1).
+  - apply H with (m := 1) (n := 2).
+    apply le_S.
+    apply le_refl.
+  - inversion H0.
+    subst.
+    inversion H3.
+Qed.
+
 (* (b) Transitivity *)
 Lemma le_trans : forall m n o, m <= n -> n <= o -> m <= o.
 Proof.
-  (* FILL IN HERE *)
-Admitted.
+  intros.
+  generalize dependent m.
+  induction H0.
+  - intros; eauto.
+  - intros.
+    inversion H; subst.
+    + constructor. assumption.
+    + constructor.
+      apply IHle.
+      constructor.
+      assumption.
+Qed.
 
-(** Exercise: *)
 (* Write an inductively-defined proposition for establishing that
    a natural number is odd, and prove that it works for the following examples.  *)
 Inductive odd : nat -> Prop :=
-(* FILL IN HERE *) .
+| odd1 : odd 1
+| oddSS : forall m, odd m -> odd (2 + m).
 
-(** Exercise: *)
 Example odd_1 : odd 1.
 Proof.
-  (* FILL IN HERE *)
-Admitted.
+  apply odd1.
+Qed.
 
-(** Exercise: *)
 Example odd_7 : odd 7.
 Proof.
-  (* FILL IN HERE *)
-Admitted.
+  repeat constructor.
+Qed.
 
-(** Exercise: *)
 Example even_0 : ~odd 0.
 Proof.
-  (* FILL IN HERE *)
-Admitted.
+  unfold not.
+  intros H.
+  inversion H.
+Qed.
 
-(** Exercise: *)
 Example even_14 : ~odd 14.
 Proof.
-  (* FILL IN HERE *)
-Admitted.
+  unfold not.
+  intros H.
+  inversion H; subst; clear H.
+  inversion H1; subst; clear H1.
+  inversion H0; subst; clear H0.
+  inversion H1; subst; clear H1.
+  inversion H0; subst; clear H0.
+  inversion H1; subst; clear H1.
+  inversion H0; subst; clear H0.
+  inversion H1; subst; clear H1.
+Qed.
 
-(** Exercise: *)
-(* Prove that an even number is never odd: *)
+(* Prove that an even numbers is never odd: *)
 Lemma even_not_not : forall (n : nat),
     even n = true ->
     ~ odd n.
 Proof.
-  (* FILL IN HERE *)
-Admitted.
+  unfold not; intros n ev_n odd_n.
+  induction odd_n.
+  - simpl in ev_n.
+    inversion ev_n.
+  - simpl in ev_n.
+    apply IHodd_n.
+    assumption.
+Qed.
 
-(** Exercise: *)
 (* Now prove that an odd numbers is never even: *)
 Lemma odd_not_even : forall (n : nat),
     odd n ->
     even n = false.
 Proof.
-  (* FILL IN HERE *)
-Admitted.
+  intros n odd_n.
+  induction odd_n.
+  - reflexivity.
+  - simpl.
+    rewrite IHodd_n.
+    reflexivity.
+Qed.
 
 (*********************************************************
   Part 3: Big-Step Operational Semantics
@@ -403,9 +398,8 @@ Module aevalR_extended.
   Reserved Notation "st 'A=[' e ']=>' n" (at level 90, left associativity).
   Reserved Notation "st 'AE=[' e ']=>' n" (at level 90, left associativity).
 
-  (** Exercise: *)
   Inductive aexpExp : Type :=
-  (* ADD CONSTRUCTOR HERE *)
+  | AEPow (a1 : aexpExp) (n : nat)
   | AENum (n : nat)
   | AEId (x : string)
   | AEPlus (a1 a2 : aexpExp)
@@ -414,11 +408,12 @@ Module aevalR_extended.
 
   (* ----------------------------------------------------------------- *)
 
-  (** Exercise: *)
-  (* The exponentiation function [pow] is in the standard library,
-  feel free to use it here. *)
+  (* The exponentiation function [pow] is in the standard library. *)
   Inductive aeevalR : state -> aexpExp -> nat -> Prop :=
-  (* FILL IN THE REDUCTION RULE FOR EXPONENTIATION HERE *)
+  (* Add the reduction rule for exponents. *)
+  | E_AEPow (st : state) (a : aexpExp) (n m: nat) :
+      (st AE=[a]=> m) ->
+      st AE=[AEPow a n]=> pow m n
   | E_AENum (st : state) (n : nat) :
       st AE=[AENum n]=> n
   | E_AEId (st : state) (x : string) :
@@ -449,18 +444,15 @@ Module aevalR_extended.
   | AMinus (a1 a2 : aexp)
   | AMult (a1 a2 : aexp).
 
-  (** Exercise: *)
-  (* Define a helper function to help translate AEPow
-     ntimes a 0 = a
-     ntimes a (S n) = a * (ntimes a n)
-*)
-  Fixpoint nTimes (a : aexp) (n : nat) : aexp :=
-    (* FILL IN HERE *) a.
+  Fixpoint powTimes (a : aexp) (n : nat) : aexp :=
+    match n with
+    | 0 => ANum 1
+    | S n' => AMult a (powTimes a n')
+    end.
 
-  (** Exercise: *)
   Fixpoint aexpExpToaexp (ae : aexpExp) : aexp :=
     match ae with
-    (* FILL IN HERE *)
+    | AEPow a1 n => powTimes (aexpExpToaexp a1) n
     | AENum n => ANum n
     | AEId x => AId x
     | AEPlus a1 a2 => APlus (aexpExpToaexp a1) (aexpExpToaexp a2)
@@ -468,8 +460,8 @@ Module aevalR_extended.
     | AEMult a1 a2 => AMult (aexpExpToaexp a1) (aexpExpToaexp a2)
     end.
 
-  (** Exercise: *)
   (* Now prove this elaboration is sound. *)
+
   Inductive aevalR : state -> aexp -> nat -> Prop :=
   | E_ANum (st : state) (n : nat) :
       st A=[ANum n]=> n
@@ -490,22 +482,23 @@ Module aevalR_extended.
 
   where "st 'A=[' a ']=>' n" := (aevalR st a n) .
 
-  (** Exercise: *)
-  (* Step One: prove that your helper function is sound. *)
   Lemma powTimesCorrect : forall st a n m,
       (st A=[ a ]=> m) ->
-      st A=[ nTimes a n ]=> m ^ n.
+      st A=[ powTimes a n ]=> m ^ n.
   Proof.
-    (* FILL IN HERE *)
-  Admitted.
+    induction n; simpl; intros.
+    - constructor.
+    - constructor; try assumption.
+      apply IHn. assumption.
+  Qed.
 
-  (** Exercise: *)
-  (* Step Two: Prove your elaboration is sound. *)
   Lemma aexpExpToaexpCorrect : forall ae st m,
       st AE=[ae]=> m -> st A=[aexpExpToaexp ae]=> m.
   Proof.
-    (* FILL IN HERE *)
-  Admitted.
+    intros.
+    - induction H; simpl; try solve [constructor; assumption].
+      apply powTimesCorrect; try assumption.
+  Qed.
 
 End aevalR_extended.
 
@@ -516,14 +509,9 @@ End aevalR_extended.
 From PLF Require Import Smallstep.
 Module LCBool.
 
-  (* Let's add booleans to the untyped lambda calculus from last
-     week's lab !*)
-
-  (* t := ...
-     | true
-     | false
-     | if t then t else t end *)
-
+  (* -- Update the syntax and CBV semantics of the Lambda calculus with booleans. *)
+  (* Let's add booleans to our
+     lambda calculus!*)
   Inductive tm : Type :=
   | tm_var   : string -> tm
   | tm_app   : tm -> tm -> tm
@@ -583,16 +571,14 @@ Hint Unfold s : core.
 (* ================================================================= *)
 (** ** Values *)
 
-(* (\x, if x then false else true end) true *)
-
-(** Exercise: *)
-(** Update the definition of values to reflect that true and false are
-    now values.  *)
+(** true and false are now values: *)
 Inductive value : tm -> Prop :=
   | v_abs : forall x t1,
       value <<{ \x, t1}>>
-  | v_true : value tm_true
-  | v_false : value <<{false}>>.
+  | v_true :
+      value <<{true}>>
+  | v_false :
+      value <<{false}>>.
 
 Hint Constructors value : core.
 
@@ -609,17 +595,13 @@ Hint Constructors value : core.
        [x:=s](\x, t)         = \x:T, t
        [x:=s](\y, t)         = \y:T, [x:=s]t         if x <> y
        [x:=s](t1 t2)         = ([x:=s]t1) ([x:=s]t2)
-       [x:=s]true            = true
-       [x:=s]false           = false
-       [x:=s](if t1 then t2 else t3 end) = if [x:=s]t1 then [x:=s]t2 else [x:=s]t3 end
 
 *)
 
+(** ... and formally: *)
+
 Reserved Notation "'[' x ':=' s ']' t" (in custom stlc at level 20, x constr).
 
-(** Exercise: *)
-(* Update the substitution function to account for booleans and if
-   expressions.*)
 Fixpoint subst (x : string) (s : tm) (t : tm) : tm :=
   match t with
   | tm_var y =>
@@ -631,7 +613,7 @@ Fixpoint subst (x : string) (s : tm) (t : tm) : tm :=
   | <<{true}>> => <<{true}>>
   | <<{false}>> => <<{false}>>
   | <<{if t1 then t2 else t3}>> =>
-    <<{if [x:=s]t1 then [x:=s]t2 else [x:=s]t3}>>
+      <<{if ([x:=s] t1) then ([x:=s] t2) else ([x:=s] t3)}>>
   end
 
 where "'[' x ':=' s ']' t" := (subst x s t) (in custom stlc).
@@ -642,8 +624,6 @@ where "'[' x ':=' s ']' t" := (subst x s t) (in custom stlc).
 (** ** Reduction *)
 
 (**
-   Here are the small-step reduction rules for our extended lambda calculus:
-
                                value v2
                      ---------------------------                     (ST_AppAbs)
                      (\x,t1) v2 --> [x:=v2]t1
@@ -659,19 +639,18 @@ where "'[' x ':=' s ']' t" := (subst x s t) (in custom stlc).
 
                            t1 --> t1'
                --------------------------
-               if t1 then t2 else t3 --> if t1' then t2 else t3
+               iter t1 zero=> cz succ=> cs --> iter t1' zero=> cz succ=> cs
 
                --------------------------
-               if true then t2 else t3 --> t2
+          iter tm_zero zero=> cz succ=> cs --> cz
 
               ----------------------------
-              if false then t2 else t3 --> t3
+          iter (tm_succ t1) z zero=> cz succ=> cs -->
+          cs (iter t1 z zero=> cz succ=> cs)
 *)
 
 Reserved Notation "t '-->' t'" (at level 40).
 
-(** Exercise: *)
-(* Extend the reduction relation with the three rules above *)
 Inductive step : tm -> tm -> Prop :=
   | ST_AppAbs : forall x t1 v2, (* <- beta reduction *)
          value v2 ->
@@ -684,17 +663,13 @@ Inductive step : tm -> tm -> Prop :=
          t2 --> t2' ->
          <<{v1 t2}>> --> <<{v1  t2'}>>
 
-  | ST_IfTrue : forall (t2 t3 : tm),
-      <<{if true then t2 else t3}>> --> t2
-
-  | ST_IfFalse : forall (t2 t3 : tm),
-      <<{if false then t2 else t3}>> --> t3
-
-  | ST_If : forall (t1 t1' t2 t3 : tm),
+  | ST_IfTrue : forall t1 t2,
+      <<{if true then t1 else t2}>> --> t1
+  | ST_IfFalse : forall t1 t2,
+      <<{if false then t1 else t2}>> --> t2
+  | ST_If : forall t1 t1' t2 t3,
       t1 --> t1' ->
-      <<{if t1 then t2 else t3}>> --> <<{if true then t2 else t3}>>
-
-    (* FILL IN HERE *)
+      <<{if t1 then t2 else t3}>> --> <<{if t1' then t2 else t3}>>
 
 where "t '-->' t'" := (step t t').
 
@@ -703,24 +678,19 @@ Hint Constructors step : core.
 Notation multistep := (multi step).
 Notation "t1 '-->*' t2" := (multistep t1 t2) (at level 40).
 
-(** Exercise: *)
 (* Write lambda expressions to calculate the and / or / not of booleans. *)
-Definition notB : tm :=
-  <<{\x, if x then false else true}>>.
 
-(** Exercise: *)
-Definition andB : tm :=
-  <<{\x, \y, if x then y else false}>>.
+Definition notB : tm := <<{\x, if x then false else true}>>.
+Definition andB : tm := <<{\x, \y, if x then y else false}>>.
+Definition orB : tm := <<{\x, \y, if x then true else y}>>.
 
-(** Exercise: *)
-Definition orB : tm :=
-  <<{\x, \y, if x then true else y}>>.
-
-(** Optional Exercise: *)
-(* Try to adapt the automation from Lab 6 to handle the rules you
-   added above; it will help with the next couple of exercises.  *)
+(* That was exhausting, and rather mechanical. Can we do better?  Yes,
+   proof automation to the rescue!  note that at each step, only one
+   evaluation rule applies. To know if a rule applies, we just need to
+   look at the shape of the goal, and (some of the time), tell if a
+   subterm is a value.  *)
 Ltac next_step :=
-  first [ apply ST_AppAbs; solve [repeat constructor]
+  first [apply ST_AppAbs; solve [repeat constructor]
         | apply ST_App2; solve [repeat constructor]
         | apply ST_App1; next_step
         | apply ST_IfTrue
@@ -731,7 +701,6 @@ Ltac normalize_lambda :=
   repeat (eapply multi_step;
           [ next_step | ]); simpl.
 
-(** Exercise: *)
 Example notB_ex :
   <<{notB true}>> -->* <<{false}>>.
 Proof.
@@ -739,7 +708,6 @@ Proof.
   apply multi_refl.
 Qed.
 
-(** Exercise: *)
 Example andb_ex :
   <<{notB (andB true false)}>> -->* <<{true}>>.
 Proof.
@@ -747,7 +715,6 @@ Proof.
   apply multi_refl.
 Qed.
 
-(** Exercise: *)
 Example orb_ex :
   <<{orB (orB true false) (notB (andB true false))}>> -->* <<{true}>>.
 Proof.
@@ -755,12 +722,11 @@ Proof.
   apply multi_refl.
 Qed.
 
-(** Exercise: *)
 Example andb_ex2 :
   <<{orB (andB true (andB true (andB true (andB true false))))
          (andB true (andB true (andB true (andB true true))))}>> -->* <<{true}>>.
 Proof.
-  normalize_lambda.
+  normalize_lambda. simpl.
   apply multi_refl.
 Qed.
 
