build-dep.sh
@@ -1,0 +1,8 @@
+curl --output lf.tgz https://softwarefoundations.cis.upenn.edu/lf-current/lf.tgz
+curl --output plf.tgz https://softwarefoundations.cis.upenn.edu/plf-current/plf.tgz
+tar -xf lf.tgz
+tar -xf plf.tgz
+cd lf
+make
+cd ../plf
+make
