build-lf.sh
@@ -1,4 +1,0 @@
-curl --output lf.tgz https://softwarefoundations.cis.upenn.edu/lf-current/lf.tgz
-tar -xf lf.tgz
-cd lf
-make
